coq/cilc2/clc_arity_spine.v
@@ -50,21 +50,21 @@ Proof.
     apply: tyhd. }
 Qed.
 
-Lemma arity_rearity_ok Γ A B I k s r t u l :
-  Γ ⊢ A : B : u -> B <: s @ l -> arity r A -> Γ ⊢ I : A : u -> r ≤ k ->
-  Γ ⊢ rearity k t I A : U @ l : U.
+Lemma arity_rearity_ok Γ A B I k s r t u l1 l2 :
+  Γ ⊢ A : B : u -> B <: s @ l1 -> arity r l2 A -> Γ ⊢ I : A : u -> r ≤ k ->
+  Γ ⊢ rearity k t I A : U @ l1 : U.
 Proof.
-  move=> ty. elim:ty k s r t l I=>{Γ A B u}.
+  move=> ty. elim:ty k s r t l1 l2 I=>{Γ A B u}.
   all: try solve[intros;
     match goal with
-    | [ H : arity _ _ |- _ ] => inv H
+    | [ H : arity _ _ _ |- _ ] => inv H
     end].
-  move=>Γ s l key k s0 r t l0 I sb ar tyI leq.
+  move=>Γ s l key k s0 r t l1 l2 I sb ar tyI leq.
   { inv ar.
     have[_ lt]:=sub_sort_inv sb.
-    have sb1 : U @ l <: U @ l0.
+    have sb1 : U @ l <: U @ l1.
     apply: sub_sort; eauto.
-    have {sb}sb2 : U @ l.+1 <: U @ l0.
+    have {sb}sb2 : U @ l.+1 <: U @ l1.
     apply: sub_sort; eauto.
     destruct k.
     apply: clc_pi.
@@ -87,7 +87,7 @@ Proof.
     eauto.
     apply: clc_axiom.
     apply: re_pure. }
-  move=>Γ A B s r t i key tyA ihA tyB ihB k s0 r0 t0 l I sb ar tyI leq.
+  move=>Γ A B s r t i key tyA ihA tyB ihB k s0 r0 t0 l1 l2 I sb ar tyI leq.
   { inv ar=>//=.
     have ty0 : A :U Γ ⊢ Var 0 : A.[ren (+1)] : U.
     { apply: clc_var.
@@ -102,16 +102,16 @@ Proof.
       apply: merge_pure; eauto. }
     have ty:=clc_app p mrg tyIw ty0.
     asimpl in ty.
-    have{}ty:=ihB _ _ _ t0 _ _ sb H0 ty leq.
+    have{}ty:=ihB _ _ _ t0 _ _ _ sb H0 ty leq.
     have[_ lt]:=sub_sort_inv sb.
-    have {}sb: U @ i <: U @ l.
+    have {}sb: U @ i <: U @ l1.
     { apply: sub_sort.
       eauto. }
     apply: clc_pi; eauto.
     apply: clc_conv; eauto.
     apply: clc_axiom.
     apply: re_pure. }
-  move=>Γ A B m s i sb tym ihm tyB _ k s0 r t l I sb' ar tyI leq.
+  move=>Γ A B m s i sb tym ihm tyB _ k s0 r t l1 l2 I sb' ar tyI leq.
   { apply: ihm; eauto.
     apply: sub_trans; eauto. }
 Qed.
@@ -122,21 +122,21 @@ Definition kpi k A B s r t :=
   | L => B
   end.
 
-Lemma rearity_spine Γ ms I A k s r t u v l :
-  arity_spine Γ A u ms (s @ l) v ->
-  arity r A ->
+Lemma rearity_spine Γ ms I A k s r t u v l1 l2 :
+  arity_spine Γ A u ms (s @ l1) v ->
+  arity r l2 A ->
   r ≤ k ->
   Γ |> U ->
   Γ ⊢ I : A : U ->
-  arity_spine Γ (rearity k t I A) U ms (kpi k (spine I ms) (t @ l) U U U) U.
+  arity_spine Γ (rearity k t I A) U ms (kpi k (spine I ms) (t @ l1) U U U) U.
 Proof.
-  move e:(s @ l)=>n tsp.
-  elim: tsp I k s r t l e=>//={Γ ms A u v n}.
-  move=>Γ A s l key tyA I k s0 r t l0 e ar leq _ tyI; subst.
+  move e:(s @ l1)=>n tsp.
+  elim: tsp I k s r t l1 l2 e=>//={Γ ms A u v n}.
+  move=>Γ A s l key tyA I k s0 r t l1 l2 e ar leq _ tyI; subst.
   { inv ar.
     destruct k=>//=.
     inv leq.
-    have sb: U @ l0 <: U @ l0.+1.
+    have sb: U @ l1 <: U @ l1.+1.
     { apply: sub_sort; eauto. }
     apply: arity_spine_nil; eauto.
     apply: clc_pi.
@@ -152,7 +152,7 @@ Proof.
     apply: clc_axiom.
     eauto. }
   move=>Γ1 Γ2 Γ hd tl A B B' s r t u l key1 tyP tyhd mrg tsp ih
-    I k s0 r0 t0 l0 e ar leq key tyI; subst.
+    I k s0 r0 t0 l1 l2 e ar leq key tyI; subst.
   { inv ar.
     have[_ key2]:=merge_pure_inv mrg key.
     have e1:=merge_pureL mrg key1.
@@ -160,7 +160,7 @@ Proof.
     subst.
     pose proof(arity_subst (hd .: ids) H0) as ar'.
     have ty0:=clc_app key mrg tyI tyhd.
-    have {}ih:=ih _ _ _ _ t0 _ erefl ar' leq key ty0.
+    have {}ih:=ih _ _ _ _ t0 _ _ erefl ar' leq key ty0.
     have ty1 : A :U Γ1 ⊢ Var 0 : A.[ren (+1)] : U.
     { apply: clc_var.
       constructor; eauto. }
@@ -171,7 +171,7 @@ Proof.
       constructor; eauto. }
     have ty2:=clc_app (key_u A key) mrg1 tyIw ty1.
     asimpl in ty2.
-    have[l1[tyA[sb[_ tyB]]]]:=pi_inv tyP.
+    have[l0[tyA[sb[_ tyB]]]]:=pi_inv tyP.
     have tyr:=arity_rearity_ok t0 tyB sb H0 ty2 leq.
     apply: arity_spine_pi; eauto.
     apply: clc_pi.
@@ -231,20 +231,20 @@ Proof.
     apply: ih; eauto. }
 Qed.
 
-Lemma ind_spine'_invX Γ A B Cs ms s t :
+Lemma ind_spine'_invX Γ A B Cs ms s t l :
   Γ |> U ->
-  arity s A ->
+  arity s l A ->
   Γ ⊢ spine' (Ind A Cs s) ms : B : t ->
-  exists A' t l,
-    arity s A' /\
-    Γ ⊢ A' : t @ l : U /\
+  exists A' t l',
+    arity s l A' /\
+    Γ ⊢ A' : t @ l' : U /\
     arity_spine Γ A U (rev ms) A' t /\
     A' <: B.
 Proof.
   move e:(spine' (Ind A Cs s) ms)=>n k a ty.
-  elim: ty A Cs ms s a e k=>{Γ B t n}.
+  elim: ty A Cs ms s l a e k=>{Γ B t n}.
   all: try solve[intros; exfalso; solve_Ind_spine'].
-  move=>Γ1 Γ2 Γ A B m n s r t _ mrg tym ihm tyn ihn A0 Cs ms s0 ar sp k.
+  move=>Γ1 Γ2 Γ A B m n s r t _ mrg tym ihm tyn ihn A0 Cs ms s0 l ar sp k.
   { move: sp. destruct ms.
     rewrite/rev/catrev=>//=.
     move=>//=e. inv e.
@@ -252,12 +252,12 @@ Proof.
     have e1:=merge_pureL mrg k1.
     have e2:=merge_pureR mrg k2.
     subst.
-    have[A'[t0[l[ar'[tyA'[sp sb]]]]]]:=ihm _ _ _ _ ar erefl k.
+    have[A'[t0[l0[ar'[tyA'[sp sb]]]]]]:=ihm _ _ _ _ _ ar erefl k.
     inv ar'.
     exfalso; solve_sub.
     move: sb=>/sub_pi_inv[eA[sB[e1[e2 e3]]]]; subst.
-    move: tyA'=>/pi_inv[l0[tyA1[sb[_ tyB0]]]].
-    exists B0.[n/]. exists U. exists l0.
+    move: tyA'=>/pi_inv[l3[tyA1[sb[_ tyB0]]]].
+    exists B0.[n/]. exists U. exists l3.
     have {}tyn : Γ1 ⊢ n : A1 : U.
     { apply: clc_conv.
       apply: conv_sub.
@@ -267,7 +267,7 @@ Proof.
       rewrite<-pure_re; eauto. }
     repeat split; eauto.
     apply: arity_subst; eauto.
-    replace (U @ l0) with (U @ l0).[n/] by autosubst.
+    replace (U @ l3) with (U @ l3).[n/] by autosubst.
     apply: substitution.
     apply: tyB0.
     apply: k.
@@ -276,28 +276,28 @@ Proof.
     rewrite rev_cons.
     apply: arity_spine_pi_rcons; eauto.
     apply: sub_subst; eauto. }
-  move=>Γ A Cs s l k ar cCs tyA ihA tyCs A0 Cs0 ms s0 ar0 sp _.
+  move=>Γ A Cs s l1 l2 k ar cCs tyA ihA tyCs A0 Cs0 ms s0 l0 ar0 sp _.
   { move: sp. destruct ms.
     rewrite/rev/catrev=>//=.
     move=>[e1 e2 e3]; subst.
-    exists A. exists U. exists l.
+    exists A. exists U. exists l2.
     repeat split; eauto.
     apply: arity_spine_nil; eauto.
     move=>//=e. }
-  move=>Γ A B m s i sb tym ihm tyB _ A0 Cs ms s0 ar sp k; subst.
-  { have{ihm}[A'[t[l[ar'[tyA'[sp sb']]]]]]:=ihm _ _ _ _ ar erefl k.
+  move=>Γ A B m s i sb tym ihm tyB _ A0 Cs ms s0 l0 ar sp k; subst.
+  { have{ihm}[A'[t[l[ar'[tyA'[sp sb']]]]]]:=ihm _ _ _ _ _ ar erefl k.
     exists A'. exists t. exists l.
     repeat split; eauto.
     apply: sub_trans; eauto. }
 Qed.
 
-Lemma ind_spine_invX Γ A B Cs ms s t :
+Lemma ind_spine_invX Γ A B Cs ms s l t :
   Γ |> U ->
-  arity s A ->
+  arity s l A ->
   Γ ⊢ spine (Ind A Cs s) ms : B : t ->
-  exists A' t l,
-    arity s A' /\
-    Γ ⊢ A' : t @ l : U /\
+  exists A' t l0,
+    arity s l A' /\
+    Γ ⊢ A' : t @ l0 : U /\
     arity_spine Γ A U ms A' t /\
     A' <: B.
 Proof.
@@ -307,11 +307,11 @@ Proof.
   rewrite revK in ty; eauto.
 Qed.
 
-Lemma ind_spine_inv Γ A Cs ms s t l :
+Lemma ind_spine_inv Γ A Cs ms s t l1 l2 :
   Γ |> U ->
-  arity s A ->
-  Γ ⊢ spine (Ind A Cs s) ms : t @ l : U ->
-  exists l, arity_spine Γ A U ms (t @ l) U /\ s = t.
+  arity s l1 A ->
+  Γ ⊢ spine (Ind A Cs s) ms : t @ l2 : U ->
+  arity_spine Γ A U ms (t @ l1) U /\ s = t.
 Proof.
   move=>k ar ty.
   have[A'[t0[l0[ar'[tyA'[sp sb]]]]]]:=ind_spine_invX k ar ty.
@@ -319,7 +319,7 @@ Proof.
   have[e _]:=sub_sort_inv sb; subst.
   have[sb' _]:=sort_inv tyA'.
   have[e lt]:=sub_sort_inv sb'; subst.
-  exists l1. eauto.
+  eauto.
   exfalso; solve_sub.
 Qed.
 
@@ -336,7 +336,7 @@ Proof.
     have[k1 k2]:=merge_pure_inv mrg k.
     have->:=merge_pureR mrg k2.
     eauto. }
-  move=>Γ A Cs s l k ar cCs tyA ihA tyCs ihCs Cs0 s0 ms _ e.
+  move=>Γ A Cs s l1 l2 k ar cCs tyA ihA tyCs ihCs Cs0 s0 ms _ e.
   { destruct ms; simpl in e; inv e.
     apply: clc_indd; eauto. }
 Qed.
