coq/cilc2/clc_ast.v
@@ -21,10 +21,10 @@ Inductive term : Type :=
 
 Notation "s @ l" := (Sort s l) (at level 30).
 
-Instance Ids_term : Ids term. derive. Defined.
-Instance Rename_term : Rename term. derive. Defined.
-Instance Subst_term : Subst term. derive. Defined.
-Instance substLemmas_term : SubstLemmas term. derive. Qed.
+#[global] Instance Ids_term : Ids term. derive. Defined.
+#[global] Instance Rename_term : Rename term. derive. Defined.
+#[global] Instance Subst_term : Subst term. derive. Defined.
+#[global] Instance substLemmas_term : SubstLemmas term. derive. Qed.
 
 Inductive All1 (P : term -> Prop) : list term -> Prop :=
 | All1_nil : All1 P nil
